tensorcore2d.to allegedly working

include/kuiper.h
@@ -142,4 +142,12 @@ cudaStream_t KPR_FRESH_STREAM() {
 	return s;
 }
 
+// A wrapper that adds a syncwarp after the store_matrix_sync, to match Kuiper's current
+// blocking tensor core store semantics
+#define KPR_STORE_MATRIX_SYNC(dst, src, ldm, layout) \ 
+	{ 
+		wmma::store_matrix_sync(dst, src, ldm, layout);
+		__syncwarp();
+	}
+
 #endif /* KUIPER_H */
