src/klas/Klas.GEMM.TensorCore2D.To.Inst.fst
@@ -1,0 +1,139 @@
+module Klas.GEMM.TensorCore2D.To.Inst
+#lang-pulse
+
+open Kuiper
+open Kuiper.Tensor
+open Kuiper.EMatrix
+open Kuiper.Array2.Strided
+open Kuiper.Tensor.Layout.Alg { l2_row_major as rm }
+open Kuiper.TensorCore
+open Kuiper.Array.Vectorized { has_vec_cpy, chunk }
+open Kuiper.Float.Casts { float_cast }
+module MS = Kuiper.Spec.GEMM
+
+module SZ = Kuiper.SizeT
+module K = Kuiper.Kernel.GEMM.TensorCore2D.To
+
+#push-options "--split_queries always --z3rlimit 40"
+inline_for_extraction noextract
+fn spec
+  // specialize
+  (et_ab et_acc et_cd : Type0)
+  {| scalar et_ab, has_vec_cpy et_ab, real_like et_ab |}
+  {| scalar et_acc, real_like et_acc |}
+  {| scalar et_cd, has_vec_cpy et_cd, real_like et_cd |}
+  {| float_cast et_cd et_acc, float_cast et_acc et_cd |}
+  (bm bn bk : szp)
+  (#_ : squash (chunk et_ab /?+ bk))
+  (#_ : squash (chunk et_ab /?+ bn))
+  (tm : szp{tm /?+ bm})
+  (tn : szp{tn /?+ bn})
+  (tk : szp{tk /?+ bk})
+  (wm : szp{wm * tm /?+ bm})
+  (wn : szp{wn * tn /?+ bn})
+  (#_ : squash (chunk et_ab * (bm/(wm*tm) * (bn/(wn*tn)) * warp_size) /?+ (bm * bk)))
+  (#_ : squash (chunk et_ab * (bm/(wm*tm) * (bn/(wn*tn)) * warp_size) /?+ (bk * bn)))
+  (#_ : squash (SZ.fits (wm * wn)))
+  (#_ : squash (SZ.fits (wm * tm)))
+  (#_ : squash (SZ.fits (wn * tn)))
+  (#_ : squash (valid_frag_et_dims et_ab FragA tm tn tk))
+  (#_ : squash (valid_frag_et_dims et_ab FragB tm tn tk))
+  (#_ : squash (valid_frag_et_dims et_acc FragAcc tm tn tk))
+  (#_ : squash (valid_frag_et_comb et_ab et_acc))
+  (#_ : squash (SZ.fits (bm*bk + (bm/(wm*tm) * (bn/(wn*tn)) * warp_size) - 1)))
+  (#_ : squash (SZ.fits (bk*bn + (bm/(wm*tm) * (bn/(wn*tn)) * warp_size) - 1)))
+  (#_ : squash ((bm/(wm*tm) * (bn/(wn*tn)) * (SZ.v warp_size)) <= max_threads))
+
+  // do not specialize
+  (rows shared cols : szp)
+  (gA : array2 et_ab (rm rows shared) { is_global gA })
+  (gB : array2 et_ab (rm shared cols) { is_global gB })
+  (gC : array2 et_cd (rm rows cols) { is_global gC })
+  (gD : array2 et_cd (rm rows cols) { is_global gD })
+  (alpha beta : et_acc)
+  (#_ : squash (aligned 16 (core gA)))
+  (#_ : squash (aligned 16 (core gB)))
+  (#eA : chest2 et_ab rows shared)
+  (#eB : chest2 et_ab shared cols)
+  (#eC : chest2 et_cd rows cols)
+  (#fA #fB #fC : perm)
+  preserves
+    cpu **
+    pure ((rows/bm) * (cols/bn) <= max_blocks) **
+    on gpu_loc (gA |-> Frac fA eA) **
+    on gpu_loc (gB |-> Frac fB eB) **
+    on gpu_loc (gC |-> Frac fC eC)
+  requires
+    pure (SZ.fits (rows * cols)) **
+    on gpu_loc (live gD)
+  ensures
+    exists* eD'.
+      on gpu_loc (gD |-> eD') **
+      pure (eD' %~ MS.mmcomb
+        (MS.rlincomb (to_real alpha) (to_real beta))
+        (to_real_matrix eC)
+        (to_real_matrix eA)
+        (to_real_matrix eB))
+{
+  tensor_pts_to_ref_located gA;
+  tensor_pts_to_ref_located gB;
+  tensor_pts_to_ref_located gC;
+  tensor_pts_to_ref_located gD;
+
+  dassert (bm %^ tm = 0sz);
+  dassert (bn %^ tn = 0sz);
+  dassert (bk %^ tk = 0sz);
+
+  dguard (rows   %^ bm = 0sz);
+  dguard (shared %^ bk = 0sz);
+  dguard (cols   %^ bn = 0sz);
+
+  lemma_divides_chain (wm * tm) bm rows;
+  lemma_divides_chain (wn * tn) bn cols;
+
+  let nblk = rows/^bm *^ (cols/^bn);
+  let nthr = bm/^(wm*^tm) *^ (bn/^(wn*^tn)) *^ warp_size;
+
+  assert pure ((rows/bm) * (cols/bn) == nblk);
+  assert pure ((rows/bm) * (cols/bn) <= max_blocks);
+  dassert (nblk <=^ SZ.uint_to_t 2097152);
+  assert pure (nblk <= max_blocks);
+
+  dassert ((bm *^ bk) %^ (chunk et_ab *^ nthr) = 0sz);
+  dassert ((bk *^ bn) %^ (chunk et_ab *^ nthr) = 0sz);
+
+  lemma_divides_trans (chunk et_ab) bk shared;
+  assert pure (chunk et_ab /?+ shared);
+  lemma_aligned_strided_row_major_l2_row_major
+    #(SZ.v rows) #(SZ.v shared) (chunk et_ab);
+
+  lemma_divides_trans (chunk et_ab) bn cols;
+  assert pure (chunk et_ab /?+ cols);
+  lemma_aligned_strided_row_major_l2_row_major
+    #(SZ.v shared) #(SZ.v cols) (chunk et_ab);
+
+  let rA = to_real_matrix eA;
+  let rB = to_real_matrix eB;
+  let rC = to_real_matrix eC;
+  let comb =
+    (fun (x : et_cd) (y : et_acc) ->
+      MS.lincomb_to #et_acc #et_cd alpha beta x y);
+  let comb_r = MS.rlincomb (to_real alpha) (to_real beta);
+  MS.lincomb_to_approx2 #et_acc #et_cd alpha beta;
+
+  #set-options "--fuel 0 --ifuel 0 --z3refresh" {
+  launch_sync (
+    K.mk_kernel comb comb_r
+      gA #eA gB #eB
+      gC #_ #eC gD #eC
+      bm bn bk tm tn tk wm wn
+      #_ #_ #_ #_ #_ #_ #_ #_
+      #fA #fB #fC
+      nblk nthr
+      #_ #_ #_ #_ #_ #_ #_ #_ #_ #_ #_ #_ #_
+      rA rB rC #_ #_ ()
+  )};
+
+  ()
+}
+#pop-options
