src/klas/Klas.GEMM.TensorCore2D.To.Inst.fsti
@@ -1,0 +1,75 @@
+module Klas.GEMM.TensorCore2D.To.Inst
+#lang-pulse
+
+open Kuiper
+open Kuiper.Tensor
+open Kuiper.EMatrix
+open Kuiper.Array2.Strided
+open Kuiper.Tensor.Layout.Alg { l2_row_major as rm }
+open Kuiper.TensorCore
+open Kuiper.Array.Vectorized { has_vec_cpy, chunk }
+open Kuiper.Float.Casts { float_cast }
+module MS = Kuiper.Spec.GEMM
+
+module SZ = Kuiper.SizeT
+
+inline_for_extraction noextract
+fn spec
+  // specialize
+  (et_ab et_acc et_cd : Type0)
+  {| scalar et_ab, has_vec_cpy et_ab, real_like et_ab |}
+  {| scalar et_acc, real_like et_acc |}
+  {| scalar et_cd, has_vec_cpy et_cd, real_like et_cd |}
+  {| float_cast et_cd et_acc, float_cast et_acc et_cd |}
+  (bm bn bk : szp)
+  (#_ : squash (chunk et_ab /?+ bk))
+  (#_ : squash (chunk et_ab /?+ bn))
+  (tm : szp{tm /?+ bm})
+  (tn : szp{tn /?+ bn})
+  (tk : szp{tk /?+ bk})
+  (wm : szp{wm * tm /?+ bm})
+  (wn : szp{wn * tn /?+ bn})
+  (#_ : squash (chunk et_ab * (bm/(wm*tm) * (bn/(wn*tn)) * 32) /?+ (bm * bk)))
+  (#_ : squash (chunk et_ab * (bm/(wm*tm) * (bn/(wn*tn)) * 32) /?+ (bk * bn)))
+  (#_ : squash (SZ.fits (wm * wn)))
+  (#_ : squash (SZ.fits (wm * tm)))
+  (#_ : squash (SZ.fits (wn * tn)))
+  (#_ : squash (valid_frag_et_dims et_ab FragA tm tn tk))
+  (#_ : squash (valid_frag_et_dims et_ab FragB tm tn tk))
+  (#_ : squash (valid_frag_et_dims et_acc FragAcc tm tn tk))
+  (#_ : squash (valid_frag_et_comb et_ab et_acc))
+  (#_ : squash (SZ.fits (bm*bk + (bm/(wm*tm) * (bn/(wn*tn)) * 32) - 1)))
+  (#_ : squash (SZ.fits (bk*bn + (bm/(wm*tm) * (bn/(wn*tn)) * 32) - 1)))
+  (#_ : squash ((bm/(wm*tm) * (bn/(wn*tn)) * 32) <= max_threads))
+
+  // do not specialize
+  (rows shared cols : szp)
+  (gA : array2 et_ab (rm rows shared) { is_global gA })
+  (gB : array2 et_ab (rm shared cols) { is_global gB })
+  (gC : array2 et_cd (rm rows cols) { is_global gC })
+  (gD : array2 et_cd (rm rows cols) { is_global gD })
+  (alpha beta : et_acc)
+  (#_ : squash (aligned 16 (core gA)))
+  (#_ : squash (aligned 16 (core gB)))
+  (#eA : chest2 et_ab rows shared)
+  (#eB : chest2 et_ab shared cols)
+  (#eC : chest2 et_cd rows cols)
+  (#fA #fB #fC : perm)
+  preserves
+    cpu **
+    pure ((rows/bm) * (cols/bn) <= max_blocks) **
+    on gpu_loc (gA |-> Frac fA eA) **
+    on gpu_loc (gB |-> Frac fB eB) **
+    on gpu_loc (gC |-> Frac fC eC)
+  requires
+    pure (SZ.fits (rows * cols)) **
+    on gpu_loc (live gD)
+  ensures
+    exists* eD'.
+      on gpu_loc (gD |-> eD') **
+      pure (eD' %~ MS.mmcomb
+        (MS.rlincomb (to_real alpha) (to_real beta))
+        (to_real_matrix eC)
+        (to_real_matrix eA)
+        (to_real_matrix eB))
+
